{
 "cells": [
  {
   "cell_type": "markdown",
   "metadata": {},
   "source": [
    "# Second order system parameters"
   ]
  },
  {
   "cell_type": "markdown",
   "metadata": {},
   "source": [
    "A second order system can be put into the form\n",
    "\n",
    "$$ \\frac{d^2 y}{dt^2} + \\frac{\\omega_0}{Q_0} \\frac{d y}{dt} + \\omega_0^2 y = b_1 \\frac{d x}{dt} + b_0 x$$\n",
    "\n",
    "Where $x(t)$ is the forcing input and $y(t)$ is the system's response"
   ]
  },
  {
   "cell_type": "markdown",
   "metadata": {},
   "source": [
    "## Laplace transform\n",
    "\n",
    "The particular solution of these systems to a unit pulse at $t=0$ can be put in the form \n",
    "\n",
    "$$ y_p(t) = y_0 e^{s_0 t} u(t) $$ \n",
    "\n",
    "Where $s_0$ is a complex number and $u(t)$ is the unit step function $u(t) = 0$ for $t<0$ and $u(t) = 1$ for $t>1$ . This is the solution for a unit pulse at $t=0$ \n",
    "\n",
    "For a general input $x(t)$ the response will be a sum of different $s$ values\n",
    "\n",
    "$$ y(t) = \\int Y(s) e^{s t} ds $$\n",
    "\n",
    "### Response in Laplace form\n",
    "\n",
    "Because any function $f(t)$ can be decomposed in a sum of decaying exponentials, both $x(t)$ and $y(t)$ can be written as in the last equation. $Y(s)$ is then the Laplace transform of $y(t)$ \n",
    "\n",
    "Also, since the differential equation is a linear system, knowing the response for all values of $s$ means that we can calculate the response to any input $x(t)$ by integrating over $s$ \n",
    "\n",
    "The Laplace response is obtained by replacing $y(t) = Y(s) e^{s t}$ and $x(t) = X(s) e^{s t} $\n",
    "\n",
    "$$ s^2 Y + s \\frac{\\omega_0}{Q_0} Y + \\omega_0^2 Y = b_1 s X + b_0 X$$\n",
    "\n",
    "so that \n",
    "\n",
    "$$ Y = \\frac{b_1 s  + b_0 }{s^2  + s \\frac{\\omega_0}{Q_0}  + \\omega_0^2 } X $$"
   ]
  },
  {
   "cell_type": "markdown",
   "metadata": {},
   "source": [
    "## Solution for unit pulse at $t=0$\n",
    "\n",
    "This is the free-oscillating solution"
   ]
  },
  {
   "cell_type": "markdown",
   "metadata": {},
   "source": [
    "Replace $y(t) \\rightarrow y_p(t)$ in the differential equation\n",
    "\n",
    "$$ s_0^2 y_0 e^{s_0 t}  + \\frac{\\omega_0}{Q_0} s_0 y_0 e^{s_0 t}  + \\omega_0^2  y_0 e^{s_0 t}  = 0$$\n",
    "\n",
    "for $t>0$, or\n",
    "\n",
    "$$ s_0^2  + \\frac{\\omega_0}{Q_0} s_0  + \\omega_0^2    = 0$$\n",
    "\n",
    "so that\n",
    "\n",
    "$$ s_0 = -\\frac{\\omega_0}{2 Q_0} \\pm \\sqrt{\\left(\\frac{\\omega_0}{2 Q_0}\\right)^2-\\omega_0^2} $$\n",
    "\n",
    "or \n",
    "\n",
    "$$ s_0 = \\omega_0 \\left( \\pm \\sqrt{\\frac{1}{4 Q_0^2}-1} - \\frac{1}{2 Q_0}\\right) $$\n",
    "\n",
    "### When $Q_0$ is large\n",
    "\n",
    "$$ s_0 = \\pm \\jmath  \\omega_f - \\frac{\\omega_0}{2 Q_0}$$\n",
    "\n",
    "with $\\omega_f = \\omega_0 \\sqrt{1-\\frac{1}{4 Q_0^2}}$, close to $\\omega_0$ for large values of $Q_0$\n",
    "\n",
    "and the solution is \n",
    "\n",
    "$$ y_p(t) = e^{- \\frac{\\omega_0}{2 Q_0} t} \\left(y_0^+  e^{+\\jmath\\omega_f t}  + y_0^-  e^{-\\jmath\\omega_f t} \\right)u(t)$$ \n",
    "\n",
    "\n",
    "### Poles\n",
    "\n",
    "The two solutions of $s_0^+ = s_0$ and $s_0^- =s_0^*$ are the poles of the response function of the system because they make its denominator $=0$"
   ]
  },
  {
   "cell_type": "markdown",
   "metadata": {},
   "source": [
    "## Amplitude of response to a unit pulse\n",
    "\n",
    "The Laplace transform of a unit pulse $x(t) = \\delta(t)$ is $X(s) = 1$ \n",
    "\n",
    "The Laplace transform of the response is then given by $Y$ by replacing $X=1$\n",
    "\n",
    "$$ Y_f = \\frac{b_1 s  + b_0 }{s^2  + s \\frac{\\omega_0}{Q_0}  + \\omega_0^2 } $$\n",
    "\n",
    "The response is the inverse Laplace transform of $Y_f$.\n",
    "\n"
   ]
  },
  {
   "cell_type": "markdown",
   "metadata": {},
   "source": [
    "### Known Laplace transforms that can be useful in our case"
   ]
  },
  {
   "cell_type": "markdown",
   "metadata": {},
   "source": [
    "| $f(t)$ | $F(s)$ |\n",
    "| :-----: | :-------: |\n",
    "| $\\delta(t)$ | $1$ |\n",
    "| $e^{s_0 t}$ | $\\frac{1}{s+s_0}$ |\n",
    "| $a f(t)$ | $a F(s)$ |\n",
    "| $f(t) + g(t) $ | $F(s)+G(s)$ |\n",
    "\n",
    "\n",
    "The fraction of polynomial functions in $Y_f$ can be represented as a linear superposition of Laplace transforms of $e^{s_0 t}$.\n",
    "\n",
    "$$ \n",
    "\\begin{align}\n",
    "Y_f & = \\frac{b_1 s  + b_0 }{s^2  + s \\frac{\\omega_0}{Q_0}  + \\omega_0^2 }  \\\\\n",
    "    & = \\frac{c_1}{s+s_0} + \\frac{c_2}{s+s_0^*} \\\\\n",
    "    & = \\frac{c_1(s+s_0^*)+ c_2(s+s_0)}{s^2+2 \\Re{(s_0)} s + |s_0|^2} \n",
    "\\end{align}\n",
    "$$\n",
    "\n",
    "The denominator just tells us what we already know, the solutions for $s_0$ found above. \n",
    "\n",
    "The numerator has to be determined independently as a function of the values of $b_1$ and $b_0$. We have\n",
    "\n",
    "$$ \n",
    "b_1 s + b_0  = (c_1+c_2) s + (c_1 s_0^* + c_2 s_0)\n",
    "$$\n",
    "\n",
    "so that \n",
    "$$\n",
    "\\begin{align}\n",
    "b_1 &=& c_1 &+& c_2 \\\\\n",
    "b_0 &=& c_1 s_0^* &+& c_2 s_0\n",
    "\\end{align}\n",
    "$$\n",
    "\n",
    "$$\n",
    "\\begin{align}\n",
    "- b_1 s_0 &= - c_1 s_0  &-& c_2 s_0  \\\\\n",
    "b_0 &= c_1 s_0^* &+& c_2 s_0\n",
    "\\end{align}\n",
    "$$\n",
    "\n",
    "$$\n",
    "b_0 - b_1 s_0  = c_1 (s_0^* - s_0) \n",
    "$$\n",
    "\n",
    "$$\n",
    "\\begin{align}\n",
    "c_1  &=  \\frac{b_0 - b_1 s_0 }{s_0^* - s_0} \\\\\n",
    "     &=  \\frac{b_0 - b_1 s_0 }{-2\\jmath\\Im(s_0)} \\\\ \n",
    "     &=  \\jmath \\frac{b_0 - b_1 s_0 }{2\\Im(s_0)} \\\\\n",
    "     &=  \\jmath \\frac{b_0 - b_1 \\Re(s_0) - \\jmath b_1 \\Im(s_0) }{2\\Im(s_0)} \\\\\n",
    "     &=  \\frac{  b_1 \\Im(s_0) + \\jmath(b_0 - b_1 \\Re(s_0))  }{2\\Im(s_0)} \\\\\n",
    "     &=    b_1  + \\jmath\\frac{(b_0 - b_1 \\Re(s_0))  }{2 \\Im(s_0)}\n",
    "\\end{align}\n",
    "$$\n",
    "\n",
    "$$\n",
    "\\begin{align}\n",
    "b_0 - b_1 s_0^*  &= c_2 (s_0 - s_0^*) \\\\\n",
    "c_2  &=  -\\jmath \\frac{b_0 - b_1 s_0^* } {2 \\Im(s_0)} \\\\\n",
    "     &=  \\frac{  b_1 \\Im(s_0) - \\jmath(b_0 - b_1 \\Re(s_0))  }{ 2 \\Im(s_0)} \\\\\n",
    "     &= c_1^*\n",
    "\\end{align}\n",
    "$$\n",
    "\n",
    "Usually either $b_0$ or $b_1$ is $0$\n",
    "\n",
    "### $b_1 = 0$\n",
    "\n",
    "$$c_1 = -c_2$$\n",
    "\n",
    "$$ c_1 (s_0 - s_0^*) = b_0 $$\n",
    "\n",
    "$$ c_1  = \\frac{b_0}{\\jmath\\Im{s_0}} $$\n",
    "$$ c_2  = -\\frac{b_0}{\\jmath\\Im{s_0}} $$\n",
    "\n",
    "### $b_0 = 0$\n",
    "\n",
    "$$ c_2 = b_1-c_1$$\n",
    "\n",
    "$$ c_1 s_0 + c_2 s_0^* = 0  $$\n",
    "\n",
    "$$ c_1 s_0 + (b_1-c_1) s_0^* = 0 $$\n",
    "\n",
    "$$ c_1 (s_0 - s_0^* ) = -b_1 s_0^* $$ \n",
    "\n",
    "$$ c_1  = -b_1 \\frac{s_0^*}{\\jmath\\Im{s_0}} $$ \n",
    "\n",
    "----\n",
    "$$ \n",
    "\\begin{align}\n",
    "c_2  &= b_1\\left(1+ \\frac{s_0^*}{\\jmath\\Im{s_0}}\\right) \\\\\n",
    "    &=   b_1\\left(\\frac{s_0 - s_0^* + s_0^*}{s_0 - s_0^*}\\right) \\\\\n",
    "    &=   b_1\\left(\\frac{s_0 }{s_0 - s_0^*}\\right) \\\\\n",
    "    &=   b_1\\left(\\frac{s_0 }{\\jmath\\Im{s_0}}\\right) \\\\\n",
    "    &= c_1^*\n",
    "\\end{align}$$ \n",
    "\n",
    "----\n",
    "\n",
    "$$ \n",
    "\\begin{align}\n",
    "Y_f & = \\frac{b_1 s  + b_0 }{s^2  + s \\frac{\\omega_0}{Q_0}  + \\omega_0^2 }  \\\\\n",
    "    & =  \\left( b_1  + \\jmath\\frac{(b_0 - b_1 \\Re(s_0))  }{2 \\Im(s_0)}\\right)\\frac{1}{s+s_0} +\n",
    "         \\left( b_1  - \\jmath\\frac{(b_0 - b_1 \\Re(s_0))  }{2 \\Im(s_0)}\\right)\\frac{1}{s+s_0^*} \n",
    "\\end{align}\n",
    "$$\n",
    "\n",
    "\n",
    "so the solution in time domain is:\n",
    "\n",
    "$$\n",
    "\\begin{align}\n",
    "y(t) & = \\left( b_1  + \\jmath\\frac{(b_0 - b_1 \\Re(s_0))  }{2 \\Im(s_0)}\\right) e^{s_0 t} &+ \n",
    "       \\left( b_1  + \\jmath\\frac{(b_0 - b_1 \\Re(s_0))  }{ 2 \\Im(s_0)}\\right) e^{-s_0 t}\n",
    "     & = e^{\\Re(s_0)}  \n",
    "\\end{align}\n",
    "$$"
   ]
  },
  {
   "cell_type": "code",
   "execution_count": null,
   "metadata": {},
   "outputs": [],
   "source": []
  }
 ],
 "metadata": {
  "kernelspec": {
   "display_name": "unsw",
   "language": "python",
   "name": "unsw"
  },
  "language_info": {
   "codemirror_mode": {
    "name": "ipython",
    "version": 3
   },
   "file_extension": ".py",
   "mimetype": "text/x-python",
   "name": "python",
   "nbconvert_exporter": "python",
   "pygments_lexer": "ipython3",
   "version": "3.8.5"
  }
 },
 "nbformat": 4,
 "nbformat_minor": 4
}
